rustfrontend/RustIRown.v
@@ -138,10 +138,6 @@ Next Obligation.
 Admitted.
 Next Obligation.
 Admitted.
-Next Obligation.
-Admitted.
-Next Obligation.
-Admitted.
 
 
 Section SMALLSTEP.
@@ -272,11 +268,11 @@ Inductive step_dropplace : state -> trace -> state -> Prop :=
     (* p is not owned, so just skip it (How to relate this case with
     RustIRsem because drop elaboration removes this place earlier in
     generate_drop_flag) *)
-    (NOTOWN: is_owned own p = false),
+    (NOTOWN: is_init own p = false),
     step_dropplace (Dropplace f None ((p, full) :: ps) k le own m) E0
       (Dropplace f None ps k le own m)
 | step_dropplace_init2: forall f p ps k le own m st (full: bool)
-    (OWN: is_owned own p = true)
+    (OWN: is_init own p = true)
     (DPLACE: st = (if full then gen_drop_place_state p else drop_fully_owned_box [p])),
     (* move p to match drop p *)
     step_dropplace (Dropplace f None ((p, full) :: ps) k le own m) E0
